Split off ExternalList.dfy, more words

Test/dafny0/List.dfy
@@ -1,316 +1,133 @@
-trait List {
-  predicate Valid()
-    reads this, Repr
-    ensures Valid() ==> this in Repr
-  ghost var Repr: set<object>
-  ghost var values: seq<int>
 
-  function method Length(): nat
-    requires Valid()
-    reads this, Repr
-    ensures Length() == |values|
-  
-  method Get(i: int) returns (res: int)
-    requires Valid()
-    requires 0 <= i < Length()
-    decreases Repr
-    ensures res == values[i]
-  
-  method Set(i: int, element: int)
-    requires Valid()
-    requires 0 <= i < Length()
-    decreases Repr
-    modifies Repr
-    ensures Valid()
-    ensures values == old(values[..i]) + [element] + old(values[i + 1..])
-    ensures fresh(Repr - old(Repr))
+module Collections {
+
+  trait {:termination false} List {
+    predicate Valid()
+      reads this, Repr
+      ensures Valid() ==> this in Repr
+    ghost var Repr: set<object>
+    ghost var values: seq<nat>
+
+    function method Length(): nat
+      requires Valid()
+      reads this, Repr
+      ensures Length() == |values|
     
-  method Add(element: int)
-    requires Valid()
-    decreases Repr
-    modifies Repr
-    ensures Valid()
-    ensures values == old(values) + [element]
-    ensures fresh(Repr - old(Repr))
-}
-
-class ArrayList extends List {
-
-  var data: array<int>
-  var length: nat
-
-  constructor() 
-    ensures Valid()
-    ensures values == []
-  {
-    data := new int[10];
-    length := 0;
-
-    values := [];
-    Repr := {this, data};
-  }
-
-  predicate Valid()
-    reads this, Repr
-    ensures Valid() ==> this in Repr
-  {
-    && Repr == {this, data}
-    && 0 < data.Length
-    && 0 <= length <= data.Length
-    && values == data[..length]
-  }
-
-  function method Length(): nat
-    requires Valid()
-    reads this, Repr
-    ensures Length() == |values|
-  {
-    length
-  }
-  
-  method Get(i: int) returns (res: int)
-    requires Valid()
-    requires 0 <= i < Length()
-    decreases Repr
-    ensures res == values[i]
-  {
-    res := data[i];
-  }
-
-  method Set(i: int, element: int)
-    requires Valid()
-    requires 0 <= i < Length()
-    decreases Repr
-    modifies Repr
-    ensures Valid()
-    ensures fresh(Repr - old(Repr))
-    ensures values == old(values[..i]) + [element] + old(values[i + 1..])
-  {
-    data[i] := element;
-
-    values := values[..i] + [element] + values[i + 1..];
-  }
-
-  method Add(element: int)
-    requires Valid()
-    decreases Repr
-    modifies Repr
-    ensures Valid()
-    ensures values == old(values) + [element]
-    ensures fresh(Repr - old(Repr))
-  {
-    if length == data.Length {
-      Grow();
-    }
-    data[length] := element;
-    length := length + 1;
-
-    values := values + [element];
-  }
-
-  method Grow() 
-    requires Valid()
-    modifies Repr
-    ensures length < data.Length
-    ensures fresh(data)
-    ensures unchanged(`length)
-    ensures values == old(values)
-    ensures Valid()
-  {
-    var oldSize := data.Length;
-    var newData := new int[2 * data.Length];
-    forall i | 0 <= i < oldSize {
-      newData[i] := data[i];
-    }
-    data := newData;
+    method Get(i: int) returns (res: nat)
+      requires Valid()
+      requires 0 <= i < Length()
+      decreases Repr
+      ensures res == values[i]
     
-    Repr := {this, data};
-  }
-}
-
-trait {:extern} ExternalList {
-
-  // TODO-RS: apply my "external invariant" strategy for ensuring externally-visible
-  // object are always Valid()
-
-  // TODO-RS: Can we make this "true" by default, so external implementations are 
-  // assumed to be always valid through things like access control and critical sections?
-  predicate Valid()
-    reads this, Repr
-    ensures Valid() ==> this in Repr
-
-  // TODO-RS: Similarly, can we assign this to {} or {this} by default somehow?
-  ghost var Repr: set<object>
-
-  // TODO-RS: figure out how to enforce that this acts like a function
-  function method Length(): int
-    requires Valid()
-    reads Repr
-    ensures Valid()
-  
-  method Get(i: int) returns (res: int)
-    requires Valid()
-    decreases Repr
-  
-  method Set(i: int, element: int)
-    requires Valid()
-    modifies Repr
-    decreases Repr
-    ensures Valid()
-    ensures fresh(Repr - old(Repr))
-  
-  method Add(element: int)
-    requires Valid()
-    modifies Repr
-    decreases Repr
-    ensures Valid()
-    ensures fresh(Repr - old(Repr))
-}
-
-class AsExternalList extends ExternalList {
-
-  var wrapped: List
-
-  constructor(wrapped: List) 
-    requires wrapped.Valid()
-    ensures Valid()
-  {
-    this.wrapped := wrapped;
-    this.Repr := {this} + wrapped.Repr;
+    method Set(i: int, element: nat)
+      requires Valid()
+      requires 0 <= i < Length()
+      decreases Repr
+      modifies Repr
+      ensures Valid()
+      ensures values == old(values[..i]) + [element] + old(values[i + 1..])
+      ensures fresh(Repr - old(Repr))
+      
+    method Add(element: nat)
+      requires Valid()
+      decreases Repr
+      modifies Repr
+      ensures Valid()
+      ensures values == old(values) + [element]
+      ensures fresh(Repr - old(Repr))
   }
 
-  predicate Valid()
-    reads this, Repr
-    ensures Valid() ==> this in Repr 
-  {
-    && wrapped in Repr
-    && Repr == {this} + wrapped.Repr
-    && wrapped in wrapped.Repr
-    && this !in wrapped.Repr
-    && wrapped.Repr <= Repr
-    && wrapped.Valid()
-  }
+  class ArrayList extends List {
 
-  function method Length(): int
-    requires Valid()
-    reads Repr
-  {
-    wrapped.Length()
-  }
-  
-  method Get(i: int) returns (res: int)
-    requires Valid()
-    decreases Repr
-  {
-    expect 0 <= i < wrapped.Length();
-    res := wrapped.Get(i);
-  }
-  
-  method Set(i: int, element: int)
-    requires Valid()
-    modifies Repr
-    decreases Repr
-    ensures Valid()
-    ensures fresh(Repr - old(Repr))
-  {
-    expect 0 <= i < wrapped.Length();
-    wrapped.Set(i, element);
-    Repr := {this} + wrapped.Repr;
-  }
-  
-  method Add(element: int)
-    requires Valid()
-    modifies Repr
-    decreases Repr
-    ensures Valid()
-    ensures fresh(Repr - old(Repr))
-  {
-    wrapped.Add(element);
-    Repr := {this} + wrapped.Repr;
-  }
-}
+    var data: array<nat>
+    var length: nat
 
-class AsList extends List {
+    constructor() 
+      ensures Valid()
+      ensures values == []
+    {
+      data := new nat[10];
+      length := 0;
 
-  var wrapped: ExternalList
+      values := [];
+      Repr := {this, data};
+    }
 
-  constructor(wrapped: ExternalList) 
-    requires wrapped.Valid()
-    ensures Valid()
-  {
-    this.wrapped := wrapped;
-    this.Repr := {this} + wrapped.Repr;
-  }
+    predicate Valid()
+      reads this, Repr
+      ensures Valid() ==> this in Repr
+    {
+      && Repr == {this, data}
+      && 0 < data.Length
+      && 0 <= length <= data.Length
+      && values == data[..length]
+    }
 
-  predicate Valid()
-    reads this, Repr
-    ensures Valid() ==> this in Repr 
-  {
-    && wrapped in Repr
-    && Repr == {this} + wrapped.Repr
-    && wrapped in wrapped.Repr
-    && this !in wrapped.Repr
-    && wrapped.Repr <= Repr
-    && wrapped.Valid()
-  }
+    function method Length(): nat
+      requires Valid()
+      reads this, Repr
+      ensures Length() == |values|
+    {
+      length
+    }
+    
+    method Get(i: int) returns (res: nat)
+      requires Valid()
+      requires 0 <= i < Length()
+      decreases Repr
+      ensures res == values[i]
+    {
+      res := data[i];
+    }
 
-  function method Length(): nat
-    requires Valid()
-    reads this, Repr
-    ensures Length() == |values|
-  {
-    var result := wrapped.Length();
-    // TODO-RS: Ideally we would include `expect result >= 0;`, but
-    // we can't currently do that in a function, even though we really want that in
-    // the compiled version.
-    assume {:axiom} result == |values|;
-    result
-  }
-  
-  method Get(i: int) returns (res: int)
-    requires Valid()
-    requires 0 <= i < Length()
-    decreases Repr
-    ensures res == values[i]
-  {
-    res := wrapped.Get(i);
-    assume {:axiom} res == values[i];
-  }
-  
-  method Set(i: int, element: int)
-    requires Valid()
-    requires 0 <= i < Length()
-    decreases Repr
-    modifies Repr
-    ensures Valid()
-    ensures values == old(values[..i]) + [element] + old(values[i + 1..])
-    ensures fresh(Repr - old(Repr))
-  {
-    wrapped.Set(i, element);
+    method Set(i: int, element: nat)
+      requires Valid()
+      requires 0 <= i < Length()
+      decreases Repr
+      modifies Repr
+      ensures Valid()
+      ensures fresh(Repr - old(Repr))
+      ensures values == old(values[..i]) + [element] + old(values[i + 1..])
+    {
+      data[i] := element;
 
-    // Presumably cheap sanity check
-    var elementAfter := wrapped.Get(i);
-    expect elementAfter == element;
+      values := values[..i] + [element] + values[i + 1..];
+    }
 
-    values := values[..i] + [element] + values[i + 1..];
-    Repr := {this} + wrapped.Repr;
-  }
+    method Add(element: nat)
+      requires Valid()
+      decreases Repr
+      modifies Repr
+      ensures Valid()
+      ensures values == old(values) + [element]
+      ensures fresh(Repr - old(Repr))
+    {
+      if length == data.Length {
+        Grow();
+      }
+      data[length] := element;
+      length := length + 1;
 
-  method Add(element: int)
-    requires Valid()
-    decreases Repr
-    modifies Repr
-    ensures Valid()
-    ensures values == old(values) + [element]
-    ensures fresh(Repr - old(Repr))
-  {
-    var lengthBefore := Length();
+      values := values + [element];
+    }
 
-    wrapped.Add(element);
-
-    values := values + [element];
-    Repr := {this} + wrapped.Repr;
-
-    expect Length() == lengthBefore + 1;
+    method Grow() 
+      requires Valid()
+      modifies Repr
+      ensures length < data.Length
+      ensures fresh(data)
+      ensures unchanged(`length)
+      ensures values == old(values)
+      ensures Valid()
+    {
+      var oldSize := data.Length;
+      var newData := new nat[2 * data.Length];
+      forall i | 0 <= i < oldSize {
+        newData[i] := data[i];
+      }
+      data := newData;
+      
+      Repr := {this, data};
+    }
   }
 }
