Test/dafny0/ExternalList.dfy
@@ -1,0 +1,206 @@
+include "./List.dfy"
+
+module ExternalCollections {
+
+  import opened Collections
+
+  trait {:extern} ExternalList {
+
+    // TODO-RS: apply my "external invariant" strategy for ensuring externally-visible
+    // object are always Valid()
+
+    // TODO-RS: Can we make this "true" by default, so external implementations are 
+    // assumed to be always valid through things like access control and critical sections?
+    predicate Valid()
+      reads this, Repr
+      ensures Valid() ==> this in Repr
+
+    // TODO-RS: Similarly, can we assign this to {} or {this} by default somehow?
+    ghost var Repr: set<object>
+
+    // TODO-RS: figure out how to enforce that this acts like a function
+    function method Length(): int
+      requires Valid()
+      reads Repr
+      ensures Valid()
+    
+    method Get(i: int) returns (res: int)
+      requires Valid()
+      decreases Repr
+    
+    method Set(i: int, element: int)
+      requires Valid()
+      modifies Repr
+      decreases Repr
+      ensures Valid()
+      ensures fresh(Repr - old(Repr))
+    
+    method Add(element: int)
+      requires Valid()
+      modifies Repr
+      decreases Repr
+      ensures Valid()
+      ensures fresh(Repr - old(Repr))
+  }
+
+  /*
+   * Adapts a Dafny-internal List as an ExternalList
+   */
+  class AsExternalList extends ExternalList {
+
+    var wrapped: List
+
+    constructor(wrapped: List) 
+      requires wrapped.Valid()
+      ensures Valid()
+    {
+      this.wrapped := wrapped;
+      this.Repr := {this} + wrapped.Repr;
+    }
+
+    predicate Valid()
+      reads this, Repr
+      ensures Valid() ==> this in Repr 
+    {
+      && wrapped in Repr
+      && Repr == {this} + wrapped.Repr
+      && wrapped in wrapped.Repr
+      && this !in wrapped.Repr
+      && wrapped.Repr <= Repr
+      && wrapped.Valid()
+    }
+
+    function method Length(): int
+      requires Valid()
+      reads Repr
+    {
+      wrapped.Length()
+    }
+    
+    method Get(i: int) returns (res: int)
+      requires Valid()
+      decreases Repr
+    {
+      expect 0 <= i < wrapped.Length();
+      res := wrapped.Get(i);
+    }
+    
+    method Set(i: int, element: int)
+      requires Valid()
+      modifies Repr
+      decreases Repr
+      ensures Valid()
+      ensures fresh(Repr - old(Repr))
+    {
+      expect 0 <= i < wrapped.Length();
+      expect 0 <= element;
+      wrapped.Set(i, element);
+      Repr := {this} + wrapped.Repr;
+    }
+    
+    method Add(element: int)
+      requires Valid()
+      modifies Repr
+      decreases Repr
+      ensures Valid()
+      ensures fresh(Repr - old(Repr))
+    {
+      expect 0 <= element;
+      wrapped.Add(element);
+      Repr := {this} + wrapped.Repr;
+    }
+  }
+
+  /*
+   * Adapts an ExternalList as a Dafny-internal List
+   */
+  class AsList extends List {
+
+    var wrapped: ExternalList
+
+    constructor(wrapped: ExternalList) 
+      requires wrapped.Valid()
+      ensures Valid()
+    {
+      this.wrapped := wrapped;
+      this.Repr := {this} + wrapped.Repr;
+    }
+
+    predicate Valid()
+      reads this, Repr
+      ensures Valid() ==> this in Repr 
+    {
+      && wrapped in Repr
+      && Repr == {this} + wrapped.Repr
+      && wrapped in wrapped.Repr
+      && this !in wrapped.Repr
+      && wrapped.Repr <= Repr
+      && wrapped.Valid()
+    }
+
+    function method Length(): nat
+      requires Valid()
+      reads this, Repr
+      ensures Length() == |values|
+    {
+      var result := wrapped.Length();
+      // TODO-RS: Ideally we would include `expect result >= 0;`, but
+      // we can't currently do that in a function, even though we really want that in
+      // the compiled version.
+      // TODO-RS: Replace with `expect {:axiom} ...` when supported.
+      assume result == |values|;
+      result
+    }
+    
+    method Get(i: int) returns (res: nat)
+      requires Valid()
+      requires 0 <= i < Length()
+      decreases Repr
+      ensures res == values[i]
+    {
+      var result := wrapped.Get(i);
+      expect 0 <= result;
+      res := result;
+      
+      // TODO-RS: Replace with `expect {:axiom} ...` when supported.
+      assume res == values[i];
+    }
+    
+    method Set(i: int, element: nat)
+      requires Valid()
+      requires 0 <= i < Length()
+      decreases Repr
+      modifies Repr
+      ensures Valid()
+      ensures values == old(values[..i]) + [element] + old(values[i + 1..])
+      ensures fresh(Repr - old(Repr))
+    {
+      wrapped.Set(i, element);
+
+      // Presumably cheap sanity check
+      var elementAfter := wrapped.Get(i);
+      expect elementAfter == element;
+
+      values := values[..i] + [element] + values[i + 1..];
+      Repr := {this} + wrapped.Repr;
+    }
+
+    method Add(element: nat)
+      requires Valid()
+      decreases Repr
+      modifies Repr
+      ensures Valid()
+      ensures values == old(values) + [element]
+      ensures fresh(Repr - old(Repr))
+    {
+      var lengthBefore := Length();
+
+      wrapped.Add(element);
+
+      values := values + [element];
+      Repr := {this} + wrapped.Repr;
+
+      expect Length() == lengthBefore + 1;
+    }
+  }
+}
