Docs/ExternalSoundness.md
@@ -6,7 +6,7 @@ We are in the process of building multiple implementations of the AWS Encryption
 
 This is somewhat uncharted territory for Dafny: it has excelled for years at verifying properties of entirely self-contained Dafny programs, especially in an educational context, but this is one of if not the first case of releasing production software based on it. Although Dafny includes an `{:extern}` attribute that enables external code to link with Dafny in various contexts, it introduces potential unsoundness if the external code does not actually match the Dafny specification. To date, the attribute has largely been used to include trusted internal implementations, so the risk and impact of unsoundness has been somewhat minimized. Our project, however, must allow for customer code to both invoke Dafny code and implement Dafny extension points.
 
-The impact of unsoundness becomes severe in this case. If a Dafny method declares a parameter of type `Foo`, for example, where `Foo` is a Dafny class, then Dafny will not allow passing a `null` value as an argument. Once this method is compiled to a target language such as C#, however, C# will allow `null` to be passed. This can lead to errors and undefined behaviour deep within the Dafny runtime, potentially far from the source of the error if the `null` value is stored and referenced at a later time. These issues will lead to a bad customer experience as it will not be clear that their code is at fault, which in turn will lead to increased operational load for our team in order to support such customers.
+The impact of unsoundness becomes severe in this case. If a Dafny method declares a parameter of type `Foo`, for example, where `Foo` is a Dafny class, then Dafny will not allow passing a `null` value as an argument. Once this method is compiled to a target language such as C#, however, C# will allow `null` to be passed. This can lead to errors and undefined behaviour deep within the Dafny runtime, potentially far from the source of the error if the `null` value is stored and referenced at a later time. These issues will lead to a bad customer experience as it will not be clear that their code is at fault, which in turn will lead to increased operational load for our team in order to support such customers. It also undermines customer trust to tout the advantages of applying formal verification to our code base, only to ship bugs in the shim code.
 
 ## Requirements
 
@@ -26,27 +26,33 @@ The impact of unsoundness becomes severe in this case. If a Dafny method declare
 
 The `{:extern}` attribute is currently quite overloaded. It can be applied to modules, traits, classes, methods and functions, and in most cases its effect is only to ensure that the names of these elements are preserved by the compiler, so that external code can reference them in some way. The details of how Dafny-generated code and manually-written external code are combined is largely left up to the specific target language. See Dafny GitHub issue [#469](https://github.com/dafny-lang/dafny/issues/469) for details.
 
-The biggest threat to soundness is that most Dafny guarantees are checked statically. A fundamental feature of Dafny is pre- and post-conditions, expressed using `requires` and `ensures` declarations respectively.
+
 
 (*** A bit about limiting the scope of what is external? ***)
 
-We should first distiguish between two different cases of linkage with external code:
+We should first distiguish between two different cases of linkage with external code, for the sake of consistent terminology:
 
 1. *External* methods, referring to methods that external code is able to invoke.
 1. *Native* methods, referring to methods that are implemented in external code.
 
 Currently, external methods may be invoked without necessarily satisfying their pre-conditions ([#461](https://github.com/dafny-lang/dafny/issues/461)) and the implementation of native methods may not necessarily satisfy their post-conditions ([#463](https://github.com/dafny-lang/dafny/issues/461)).
 
-(*** Justify combining these concepts? ***)
+In practice, it is difficult if not impossible to ensure that a method can be implemented in external code yet not invoked from external code. For example, it is natural for a Dafny code base to define a trait that is compiled to a C# interface, which can then be implemented using a C# class. There is nothing to stop other client code from creating this class and invoking its methods. In addition, there will be frequent use cases for methods that need to support both external invocation and native implementations anyway, such as the `List` example in this doc. Therefore, we propose focussing on this use case first. This is a two-way door: we can always support external-only or native-only methods in a future release of Dafny if that is truly needed.
 
-Most issues can be addressed by forbidding all elements of Dafny method declarations that cannot be directly compiled to elements in the target language:
+The biggest threat to soundness is that most Dafny guarantees are checked statically. A fundamental feature of Dafny is pre- and post-conditions, expressed using `requires` and `ensures` declarations respectively. Most issues can be addressed by forbidding all elements of Dafny method declarations that cannot be directly compiled to elements in the target language:
 
-1. Disallow subtypes as in or out parameters.
-1. Disallow preconditions 
+1. Disallow any and all preconditions and postconditions.
+1. Disallow unbounded and/or infinite precision numeric types as in or out parameters, instead requiring concrete subtypes supported by the target language or Dafny runtime library for that language.
+1. Disallow all other subtypes as in or out parameters.
+1. Enforce all reference types used as in or out parameters must be nullable (i.e. `Foo?` rather than just `Foo`).
 
 ### Object Invariants
 
 Many other programming languages ensure object invariants through a combination of access control (making fields private so that all access and mutation happens only within a bounded set of methods) and concurrency control (to ensure only one thread can ever observe an object in an invalid state at one time). This ensures that objects are valid by default. Dafny instead approaches this by validating that any operation that requires an object to be valid (which in practice is nearly all of them) provides proof that this is true, based on the context of the operation. Thus Dafny objects are assumed invalid unless proven valid.
+
+Because of this, disallowing all preconditions on external methods is extremely limiting: it means that absolutely nothing can be assumed about any Dafny objects in the control flow of external methods. It is often not possible to dynamically verify a predicate such as `Valid()` since it usually refers to ghost state, and even if it was possible would often be prohibitively expensive. It is also dangerous, however, to allow external methods to assume objects are in a `Valid()` state without proof, for the same reasons that we cannot allow stray `null` values to pollute the Dafny runtime.
+
+If we assume and/or enforce certain invariants about the linkage between Dafny and external code, however, it is possible 
 
 ```dafny
 class Foo {
@@ -101,7 +107,7 @@ Since native implementations will be able to turn around and invoke any external
 forall m: ExternMethod, n: NativeMethod :: n.requires() ==> m.requires()
 ```
 
-In practice, it is difficult if not impossible to ensure that a method can be implemented in external code yet not invoked from external code. For example, it is natural for a Dafny code base to define a trait that is compiled to a C# interface, which can then be implemented using a C# class. There is nothing to stop other client code from creating this class and invoking its methods.
+
 
 If we assume `ExternMethod == NativeMethod`:
 
